Change execution to flatter relation structure (Part 11)
Reestablished proof of progress.

src/ReactorModel/Execution/Theorems/Progress.lean
@@ -5,53 +5,35 @@ open Reactor Classical
 
 namespace Execution
 
-variable [Proper α] [Reactor.Finite α] {rtr : α} {s : State.Over rtr} 
-
-def Step.Time.construct (ht : ¬s.Terminal) (hc : s.Closed) : (s' : State α) × (s ↓ₜ s') :=
-  let g := State.Terminal.not_elim ht |>.resolve_left (not_not.mpr hc)
-  let s' := ⟨refresh s.rtr (s.actions g.choose), g.choose, ∅, s.events⟩
-  ⟨s', hc, g.choose_spec, refresh_correct _ $ Partial.mapIdx_ids ..⟩
-
-def Step.construct (a : Dependency.Acyclic rtr) (hc : ¬s.Closed) : (s' : State α) × (s ↓ s') := 
-  let rcn := s.allowed a hc
-  if h : s.Triggers rcn
-  then ⟨_, .exec ⟨rcn.property, h, Step.Apply.RTC.construct s.toState (s.output rcn) |>.snd⟩⟩
-  else ⟨_, .skip ⟨rcn.property, h⟩⟩ 
-
--- A reactor has the progress property, if from any nonterminal state based at that reactor, we can 
+-- A reactor `rtr` has the progress property, if from any nonterminal state based at `rtr`, we can 
 -- perform an execution step.
 def Progress [Indexable α] (rtr : α) : Prop :=
   ∀ (s : State.Over rtr), ¬s.Terminal → ∃ s' : State α, Nonempty (s ↓ s')    
 
 namespace Progress
-
-theorem to_deps_acyclic_nontriv (nontriv : rtr[.rcn].Nonempty) (p : Progress rtr) : 
-    Dependency.Acyclic rtr := by
+theorem to_deps_acyclic [Indexable α] {rtr : α} (p : Progress rtr) : Dependency.Acyclic rtr := by
   simp [Dependency.Acyclic.iff_mem_acyclic]
   intro rcn hm
-  let s : State α := { rtr, tag := 0, progress := ∅, events := ∅ }
-  have n : s.Nontrivial := nontriv
-  have hc : ¬s.Closed := (Set.not_nonempty_empty $ ·.progress_nonempty n)
-  have ⟨_, e⟩ := p ⟨s, rfl, by simp, sorry⟩ (State.Terminal.not_of_not_closed hc)
-  have ⟨e⟩ := e.resolve_close hc 
-  exact e.acyclic $ e.progress_empty_mem_rcns_iff rfl |>.mpr hm
+  have ⟨_, ⟨e⟩⟩ := p _ $ State.Over.forcing_not_terminal hm
+  cases e
+  case time e => exact State.Over.forcing_not_time_step e hm |>.elim
+  case skip e => exact State.Over.forcing_skip_step_rcn_eq e ▸ e.allows_rcn.acyclic 
+  case exec e => exact State.Over.forcing_exec_step_rcn_eq e ▸ e.allows_rcn.acyclic 
 
-theorem to_deps_acyclic : (Progress rtr) → Dependency.Acyclic rtr :=
-  if h : rtr[.rcn].Nonempty 
-  then to_deps_acyclic_nontriv h 
-  else fun _ => Dependency.Acyclic.of_trivial (Partial.Nonempty.not_to_empty h)
+variable [Proper α] [Reactor.Finite α] {rtr : α} 
 
-theorem of_deps_acyclic (a : Dependency.Acyclic rtr) : Progress rtr := by
-  intro s ht
-  if hc : s.Closed then 
-    have ⟨_, a⟩ := Advance.of_nonterminal_closed ht hc
-    exact ⟨_, .advance a⟩
-  else 
-    have ⟨_, ⟨e⟩⟩ := Instantaneous.ClosedExecution.of_acyclic_not_closed a hc
-    exact ⟨_, .close e⟩
+theorem of_deps_acyclic (a : Dependency.Acyclic rtr) : Progress rtr :=
+  fun s ht =>
+    if hc : s.Closed then 
+      let ⟨_, hg⟩ := State.Terminal.not_elim ht |>.resolve_left (not_not.mpr hc)
+      ⟨_, ⟨.time ⟨hc, hg, refresh_correct _ $ Partial.mapIdx_ids ..⟩⟩⟩ 
+    else 
+      let ⟨rcn, hr⟩ := s.exists_allowed_of_acyclic_not_closed a hc
+      if h : s.Triggers rcn
+      then ⟨_, ⟨.exec ⟨hr, h, Step.Apply.RTC.construct .. |>.snd⟩⟩⟩
+      else ⟨_, ⟨.skip ⟨hr, h⟩⟩⟩
 
 theorem iff_deps_acyclic : (Progress rtr) ↔ (Dependency.Acyclic rtr) :=
   ⟨to_deps_acyclic, of_deps_acyclic⟩
 
-end Progress
-end Execution
+end Execution.Progress
